examples/sha3/proofs/Aeneas/USize64.lean
@@ -234,7 +234,14 @@ theorem USize64.ofNat_sub {a b : Nat} (hab : b ≤ a) : USize64.ofNat (a - b) = 
 @[simp] protected theorem USize64.sub_add_cancel (a b : USize64) : a - b + b = a :=
   USize64.toBitVec_inj.1 (BitVec.sub_add_cancel _ _)
 
+
+theorem USize64.lt_ofNat_iff {n : USize64} {m : Nat} (h : m < size) : n < ofNat m ↔ n.toNat < m := by
+  rw [lt_iff_toNat_lt, toNat_ofNat_of_lt' h]
+theorem USize64.ofNat_lt_iff {n : USize64} {m : Nat} (h : m < size) : ofNat m < n ↔ m < n.toNat := by
+  rw [lt_iff_toNat_lt, toNat_ofNat_of_lt' h]
 theorem USize64.le_ofNat_iff {n : USize64} {m : Nat} (h : m < size) : n ≤ ofNat m ↔ n.toNat ≤ m := by
+  rw [le_iff_toNat_le, toNat_ofNat_of_lt' h]
+theorem USize64.ofNat_le_iff {n : USize64} {m : Nat} (h : m < size) : ofNat m ≤ n ↔ m ≤ n.toNat := by
   rw [le_iff_toNat_le, toNat_ofNat_of_lt' h]
 
 /-!
