examples/sha3/proofs/Sha3/Equivalence.lean
@@ -13,9 +13,9 @@ set_option mvcgen.warning false
 
 set_option trace.Hax.hax_mvcgen_at true
 
-attribute [spec] KeccakState.Insts.CoreOpsIndexIndexPairUsizeUsizeT.index
-attribute [spec] get_ij
-attribute [spec] U64.Insts.Sha3KeccakItem1.xor_constant _veorq_n_u64 KeccakState.set set_ij
+-- attribute [spec] KeccakState.Insts.CoreOpsIndexIndexPairUsizeUsizeT.index
+-- attribute [spec] get_ij
+-- attribute [spec] U64.Insts.Sha3KeccakItem1.xor_constant _veorq_n_u64 KeccakState.set set_ij
 
 theorem iota_spec
   (st : KeccakState U64.Insts.Sha3KeccakItem1) (i : Std.Usize)
@@ -23,33 +23,24 @@ theorem iota_spec
     ⦃ ⌜ True ⌝ ⦄
     iota st i
     ⦃ ⇓ r => ⌜ (_ensures_iota st i r).holds ⌝ ⦄ := by
-  hax_mvcgen [iota, KeccakState.iota, _requires_iota]
-  mspec
-  mspec
-  sorry
-  hax_mvcgen
-  mspec
-  sorry
-  hax_mvcgen
-  mspec
-  sorry
-  hax_mvcgen
-  mspec
-  mspec
-  sorry
-  hax_mvcgen
-  mspec
-  mspec
-  hax_mvcgen
-  mspec
-  mspec
-  sorry
-  hax_mvcgen
-  mspec
-  sorry
-  hax_mvcgen
-  mspec
-  sorry
-  hax_mvcgen
-  mspec
-  sorry
+  unfold iota KeccakState.iota  KeccakState.Insts.CoreOpsIndexIndexPairUsizeUsizeT.index get_ij
+    _requires_iota at *
+  dsimp only [U64.Insts.Sha3KeccakItem1.xor_constant, _veorq_n_u64, KeccakState.set, set_ij, _ensures_iota,
+    reference.iota]
+  mvcgen
+  · grind
+  · grind
+  · hax_mvcgen at h
+    simp only [Std.Slice.len, Std.Array.to_slice, USize64.reduceToNat, decide_eq_true_eq,
+      ExceptConds.fst_false, SPred.down_pure, imp_false, USize64.not_lt]
+    rwa [USize64.ofNat_le_iff]
+    grind
+  · grind
+  · grind
+  · unfold Result.holds
+    mvcgen
+    · grind
+    · grind
+    · grind
+    · unfold ROUNDCONSTANTS reference.ROUND_CONSTANTS at *
+      grind
